{-# OPTIONS --without-K --exact-split #-}
open import logic
open import types
open import eq

-- lambda style predecessor
pred' : â„• â†’ â„•
pred' n = snd (pred'' n) where
          pred'' : â„• â†’ â„• Ã— â„•
          pred'' zero = (zero , zero)
          pred'' (suc n) = (suc (fst (pred'' n)) , fst (pred'' n))

pred : â„• â†’ â„•
pred 0       = 0
pred (suc n) = n

suc-cancel : {x y : â„•} â†’ suc x ï¼ suc y â†’ x ï¼ y
suc-cancel = ap pred

â„•-decidable-equality : has-decidable-equality â„•
â„•-decidable-equality 0 0       = (inl (refl 0))
â„•-decidable-equality 0 (suc b) = inr ((suc-neq-zero b) â‰ â»Â¹)
â„•-decidable-equality (suc a) 0 = inr (suc-neq-zero a)
â„•-decidable-equality (suc a) (suc b) = f (â„•-decidable-equality a b)
  where
    f : decidable (a ï¼ b) â†’ decidable (suc a ï¼ suc b)
    f = ï¼‹-ind (Î» (x : (decidable (a ï¼ b))) â†’ decidable (suc a ï¼ suc b))
        (Î» (p : a ï¼ b) â†’ inl (ap suc p))
        (Î» (f : a â‰  b) â†’ inr (f âˆ˜ suc-cancel))

-- inequality TODO prove this is equivalent to other one
_â‰¼_ : â„• â†’ â„• â†’ Set
x â‰¼ y = Î£ z ê‰ â„• , ((x + z) ï¼ y)

infix 4 _â‰¼_

-- partial order of â‰¤
-- 0     â‰¤ y     = ğŸ™
-- suc x â‰¤ 0     = ğŸ˜
-- suc x â‰¤ suc y = x â‰¤ y

â‰¤-refl : (n : â„•) â†’ (n â‰¤ n)
â‰¤-refl 0       = â‹†
â‰¤-refl (suc n) = â‰¤-refl n

â‰¤-trans : (l m n : â„•) â†’ (l â‰¤ m) â†’ (m â‰¤ n) â†’ (l â‰¤ n)
â‰¤-trans 0 l n _ _ = â‹†
â‰¤-trans (suc l) 0       0       p q = p
â‰¤-trans (suc l) 0       (suc n) p q = âŠ¥-rec (suc l â‰¤ suc n) p
â‰¤-trans (suc l) (suc m) 0       p q = q
â‰¤-trans (suc l) (suc m) (suc n) p q = â‰¤-trans l m n p q

â‰¤-anti : (m n : â„•) â†’ m â‰¤ n â†’ n â‰¤ m â†’ m ï¼ n
â‰¤-anti 0       0       p q = refl 0
â‰¤-anti 0       (suc n) p q = âŠ¥-rec (0 ï¼ suc n) q
â‰¤-anti (suc m) 0       p q = âŠ¥-rec (suc m ï¼ 0) p
â‰¤-anti (suc m) (suc n) p q = ap suc (â‰¤-anti m n p q)

-- strict inequality
_<_ _>_ : â„• â†’ â„• â†’ Set
x < y = suc x â‰¤ y
x > y = suc y â‰¥ x
infix 4 _<_ _>_

-- associativity of addition
+-assoc : (x y z : â„•) â†’ ((x + y) + z) ï¼ (x + (y + z))
+-assoc 0       y z = refl (y + z)
+-assoc (suc x) y z = ap suc (+-assoc x y z)

-- commutativity of addition
add-commutes0 : (n : â„•) â†’ (n + 0) ï¼ n
add-commutes0 0 =
  begin
    0 + 0 =âŸ¨âŸ© 0
  âˆ
add-commutes0 (suc n) =
  begin
                                  suc n  + 0
    =âŸ¨âŸ©                           suc (n + 0)
    =âŸ¨ ap suc (add-commutes0 n) âŸ© suc n        -- induction hypothesis
  âˆ

add-commutes-sucr : (m n : â„•) â†’ suc (m + n) ï¼ (m + suc n)
add-commutes-sucr 0 n =
  begin
        suc (0 + n)
    =âŸ¨âŸ© suc n
    =âŸ¨âŸ© 0 + suc n
  âˆ
add-commutes-sucr (suc m) n =
  begin
                                        suc (suc m  + n)
    =âŸ¨âŸ©                                 suc (suc (m + n))
    =âŸ¨ ap suc (add-commutes-sucr m n) âŸ© suc (m + suc n)
    =âŸ¨âŸ©                                 suc m  + suc n
  âˆ

add-commutes : (m n : â„•) â†’ (m + n) ï¼ (n + m)
add-commutes 0 n =
  begin
                              0 + n
    =âŸ¨âŸ©                       n
    =âŸ¨ (add-commutes0 n) â»Â¹ âŸ© n + 0
  âˆ
add-commutes (suc m) n =
  begin
                                   suc m  + n
    =âŸ¨âŸ©                            suc (m + n)
    =âŸ¨ ap suc (add-commutes m n) âŸ© suc (n + m)
    =âŸ¨ add-commutes-sucr n m âŸ©     n + suc m
  âˆ

-- cancellation
+-cancel : (x y z : â„•) â†’ (x + y ï¼ x + z) â†’ (y ï¼ z)
+-cancel 0       y z p = p
+-cancel (suc x) y z p = (+-cancel x y z (ap pred p))

-- subtraction TODO prove inverse theorems


-- multiples
data Multiple : â„• â†’ â„• â†’ Set where
  div-zero : (k : â„•) â†’ Multiple k 0
  div-suck : {n k : â„•} â†’ Multiple k n â†’ Multiple k (n + k) -- oops!

test-multiple : Multiple 3 6
test-multiple = div-suck (div-suck (div-zero 3))

div-coe : {a b k : â„•} â†’ Multiple k (a + b) â†’ Multiple k (b + a)
div-coe {a} {b} {k} m = È· (Multiple k) (add-commutes a b) m

div-fourâ†’div-two : {n : â„•} â†’ Multiple 4 n â†’ Multiple 2 n
div-fourâ†’div-two (div-zero .4) = div-zero 2
div-fourâ†’div-two (div-suck {k} {4} p) =
  (div-coe {4} {k}
   (div-coe {2 + k} {2}
    (div-suck {2 + k} {2}
     (div-coe {k} {2}
      (div-suck {k} {2} (div-fourâ†’div-two p))))))
